transc/ArTanH.v
@@ -315,16 +315,15 @@ Proof.
 Qed.
 
 (** PowerSeries for the Inverse Hyperbolic Tangent Function. *)
-Lemma ArTanH_series_coef_lemma : forall (R:COrdField) n, odd n -> (nring (R:=R) n)[#][0].
+Lemma ArTanH_series_coef_lemma : forall (R:COrdField) n, Nat.Odd n -> (nring (R:=R) n)[#][0].
 Proof.
- intros R [|n] H.
-  exfalso.
-  inversion H.
+ intros R [|n] H%Nat.Odd_OddT;
+  [destruct H as [k H]; rewrite Nat.add_1_r in H; discriminate H |].
  apply nringS_ap_zero.
 Qed.
 
 Definition ArTanH_series_coef (n:nat) :=
-match (even_odd_dec n) with
+match (Nat.Even_Odd_dec n) with
 | left _ => [0]
 | right H => [1][/](nring n)[//](ArTanH_series_coef_lemma IR n H)
 end.
@@ -349,10 +348,11 @@ Proof.
    Log_series_coef n[*]([1][-]x[-][1])[^]n)[=] ArTanH_series_coef n[*]nexp IR n (x[-][0])).
  unfold ArTanH_series_coef.
  destruct n as [|n].
-  destruct (even_odd_dec 0) as [A|A]; try inversion A.
-  simpl; rational.
+  destruct (Nat.Even_Odd_dec 0) as [A|A]; 
+  [simpl; rational |
+    exfalso; destruct A as [k B]; rewrite Nat.add_1_r in B; discriminate B ].
  rstepl (Half (R:=IR)[*] (Log_series_coef (S n)[*](x[^]S n[-]([--]x)[^]S n))).
- destruct (even_odd_dec (S n)) as [A|A]; unfold cg_minus.
+ destruct (Nat.Even_Odd_dec (S n)) as [A|A]; unfold cg_minus.
   csetoid_rewrite (inv_nexp_even _ x _ A).
   rational.
  csetoid_rewrite (inv_nexp_odd _ x _ A).
@@ -361,7 +361,8 @@ Proof.
  apply mult_wd;[|change (x[^]S n[=](x[+][--][0])[^]S n); rational].
  unfold Log_series_coef.
  apply div_wd; try apply eq_reflexive.
- csetoid_rewrite (inv_nexp_even IR [1] _ (even_S _ A)).
+ apply Nat.Even_succ in A.
+ csetoid_rewrite (inv_nexp_even IR [1] _ A).
  algebra.
 Qed.
 
